Minor changes to finish the merge/make it build.

Kami/Ex/Timing/LabelDecomposition.v
@@ -1,58 +1,114 @@
 Require Import Bool List String Omega.
 Require Import Structures.Equalities Program.Equality Eqdep Eqdep_dec.
 Require Import FunctionalExtensionality.
-Require Import Lib.Word Lib.CommonTactics Lib.ilist Lib.FMap Lib.StringEq Lib.VectorFacts Lib.Struct.
-Require Import Kami.Syntax Kami.Semantics Kami.Decomposition.
+Require Import Lib.CommonTactics Lib.FMap Lib.Struct.
+Require Import Kami.Syntax Kami.Semantics.
 
-Section GivenModule.
-  Variable m: Modules.
+Ltac shatter := repeat match goal with
+                       | [ H : exists _, _ |- _ ] => destruct H
+                       | [ H : _ /\ _ |- _ ] => destruct H
+                       end.
 
-  Section GivenOldregs.
-    Variable o: RegsT.
 
-    Variable Prule : MethsT -> Prop.
-    Variable Pmeth : MethsT -> Prop.
+Module Type Assumptions.
+  
+  Parameter m: Modules.
+  
+  Parameter Prule : MethsT -> Prop.
+  Parameter Pmeth : MethsT -> Prop.  
+  
+  Axiom Pmeth_empty : Pmeth ([])%fmap.
 
-    Example rqMeth := "rqFromProc" : String.string.
-    Example rsMeth := "rsToProc" : String.string.
-    Example Qrule := fun cs => FMap.M.find (elt := {x : SignatureT & SignT x}) rqMeth cs = None \/
-                            FMap.M.find (elt := {x : SignatureT & SignT x}) rsMeth cs = None.
-    Example Qmeth := fun cs => FMap.M.find (elt := {x : SignatureT & SignT x}) rqMeth cs = None /\
-                            FMap.M.find (elt := {x : SignatureT & SignT x}) rsMeth cs = None.
+  Axiom Prule_empty : Prule ([])%fmap.
+  
+  Axiom Prules : forall k a, List.In {| attrName := k; attrType := a |} (getRules m) ->
+                        forall o u cs retVal, SemAction o (a type) u cs retVal ->
+                                       Prule cs.
 
-    Axiom Prule_empty : Prule ([])%fmap.
-   
-    Axiom Prules : forall k a, List.In {| attrName := k; attrType := a |} (getRules m) ->
-                          forall u cs retVal, SemAction o (a type) u cs retVal ->
-                                         Prule cs.
-    Axiom Pmeths :  forall f, In f (getDefsBodies m) ->
-                         forall (u : UpdatesT) (cs : MethsT) (argV : type (arg (projT1 (attrType f)))) (retV : type (ret (projT1 (attrType f)))),
-                           SemAction o (projT2 (attrType f) type argV) u cs retV ->
-                           Pmeth cs.
+  Axiom Pmeths :  forall f, In f (getDefsBodies m) ->
+                       forall o (u : UpdatesT) (cs : MethsT) (argV : type (arg (projT1 (attrType f)))) (retV : type (ret (projT1 (attrType f)))),
+                         SemAction o (projT2 (attrType f) type argV) u cs retV ->
+                         Pmeth cs.
+  
+  Axiom Prume : forall rcs, Prule rcs ->
+                       forall mcs, Pmeth mcs ->
+                              Prule (M.union rcs mcs).  
+  
+  Axiom Pmeru : forall mcs, Pmeth mcs ->
+                       forall rcs, Prule rcs ->
+                              Prule (M.union mcs rcs).  
 
-    Axiom Pmeru : forall rcs, Prule rcs ->
-                         forall mcs, Pmeth mcs ->
-                                Prule (M.union rcs mcs).
+  Axiom Pmeme : forall mcs, Pmeth mcs ->
+                       forall mcs', Pmeth mcs' ->
+                               Pmeth (M.union mcs mcs').
+
+  Axiom Prsub : forall rcs rcs', Prule rcs' -> M.Sub rcs rcs' -> Prule rcs.
+
+End Assumptions.
+
+Module Conclusions (A : Assumptions).
+  Import A.
+
+  Lemma Pmeth_rule : forall cs, Pmeth cs -> Prule cs.
+  Proof.
+    intros. replace cs with (M.union [] cs)%fmap by (apply M.union_empty_L).
+    apply Prume. apply Prule_empty. assumption.
+  Qed.
+  
+  Fixpoint combineAll {o} (ss : Substeps m o) : MethsT :=
+    match ss with
+    | nil => []%fmap
+    | s :: ss' => M.union (cms s) (combineAll ss')
+    end.
+  
+  Definition PSubstepRec {o} (s : SubstepRec m o) : Prop :=
+    match (unitAnnot s) with
+    | Rle _ => Prule (cms s)
+    | Meth _  => Pmeth (cms s)
+    end.
+  
+  
+  Lemma basic : forall {o}, forall s : SubstepRec m o, PSubstepRec s.
+  Proof.
+    intros o s. destruct s. inversion substep; subst; unfold PSubstepRec; simpl.
+    - apply Prule_empty.
+    - apply Pmeth_empty.
+    - eapply Prules; try eassumption.
+    - eapply Pmeths; try eassumption.
+  Qed.
+  
+  Lemma PSubsteps : forall {o} (ss : Substeps m o), substepsComb ss -> (Prule (combineAll ss) /\ exists s k, In s ss /\ (unitAnnot s) = Rle k) \/ Pmeth (combineAll ss).
+  Proof. induction 1; simpl.
+         right. apply Pmeth_empty.           
+         destruct IHsubstepsComb.
+         - left. shatter. specialize (H0 _ H2). inv H0. shatter.
+           destruct H5.
+           + pose proof (basic s) as X.  unfold PSubstepRec in X; rewrite H5 in X.
+             split. apply Pmeru; assumption.
+             eauto.
+           + congruence.
+         - pose proof (basic s) as X. unfold PSubstepRec in X. destruct (unitAnnot s) eqn:Hua.
+           + left. split. apply Prume; assumption. eauto.
+           + right. apply Pmeme; assumption.
+  Qed.
+
     
-    
-    Goal forall u l, Step m o u l -> Prule (calls l).
-      induction 1. unfold hide.
-      induction ss; simpl.
-      - match goal with
-          [ |- Prule ?x ] => idtac x; change x with (@M.Map.empty {z : SignatureT & SignT z})
-        end; apply Prule_empty.
-      - destruct a. assert (Prule cms).
-        { destruct substep.
-          + apply Prule_empty.
-          + apply Prule_empty.
-          + eapply Prules; eassumption.
-          + replace (cs) with (M.union [] cs)%fmap by (apply M.union_empty_L).
-            eapply Pmeru. apply Prule_empty.
-            eapply Pmeths; eassumption.
-        }
-        simpl in IHss. inv HSubsteps. specialize (IHss H2). simpl in HWellHidden.
+  Lemma combine_compat:
+    forall {o}, forall ss : Substeps m o, combineAll ss = calls (foldSSLabel ss).
+  Proof.
+    induction ss; auto. 
+    simpl. 
+    unfold addLabelLeft. unfold getSLabel.
+    destruct a; destruct unitAnnot; simpl; destruct (foldSSLabel ss) eqn:H; simpl; simpl in IHss; congruence.
+  Qed.
+         
+  Theorem Prule_Step :  forall o u l, Step m o u l -> Prule (calls l).
+    induction 1.
+    pose (PSubsteps ss HSubsteps) as H.
+    unfold hide; simpl. destruct H; shatter;
+                          eapply Prsub; try apply M.subtractKV_sub.
+    rewrite <- combine_compat; assumption.
+    rewrite <- combine_compat; apply Pmeth_rule; assumption.
+  Qed.
 
-        (*unfold wellHidden in HWellHidden.
-        RefinementFacts.DomainSubset_KeysDisj*)
-        
-                                        
+End Conclusions.
