Kami/Ex/ProcFDInl.v
@@ -29,7 +29,7 @@ Section Inlined.
   Variable (d2eElt: Kind).
   Variable (d2ePack:
               forall ty,
-                Expr ty (SyntaxKind (Bit 2)) -> (* opTy *)
+                Expr ty (SyntaxKind (Bit optypeBits)) -> (* opTy *)
                 Expr ty (SyntaxKind (Bit rfIdx)) -> (* dst *)
                 Expr ty (SyntaxKind (Bit addrSize)) -> (* addr *)
                 Expr ty (SyntaxKind (Data dataBytes)) -> (* val1 *)
